switching to std++ maps, but some issues (#14)

theories/abs_functional_metatheory.v
@@ -18,72 +18,40 @@ Hypothesis (vars_well_typed: forall (x_:x) (G0: G) T0,
              lookup x_ G0 = Some T0 ->
              exists T_, T0 = ctxv_T T_).
 
-Definition subG (G1 G2 : G) : Prop :=
-  forall (key : string) (elt : ctxv),
-    lookup key G1 = Some elt ->
-    lookup key G2 = Some elt.
-
-Notation "G ⊢ e : T" := (typ_e G e T) (at level 5).
-Notation "G F⊢ F" := (typ_F G F) (at level 5).
-
-Lemma subG_refl: forall G0,
-  subG G0 G0.
-Proof. easy. Qed.
-
-Lemma subG_add: forall G0 G1 y T_,
-  subG G0 G1 ->
+Lemma subG_add: forall (G0 G1: G) y T_,
+  G0 ⊆ G1 ->
   G0 !! y = None ->
-  subG G0 (insert y T_ G1).
+  G0 ⊆ (insert y T_ G1).
+Proof. intros; by apply insert_subseteq_r. Qed.
+
+Lemma subG_add_2: forall (G0 G1: G) y T_,
+  subseteq G0 G1 ->
+  G0 !! y = Some T_ ->
+  subseteq G0 (insert y T_ G1).
 Proof.
   intros.
-  intros ?x_ ?T_ ?.
+  intros ?x_.
 
   destruct (eq_x y x_); subst.
-  - setoid_rewrite H0 in H1.
-    inv H1.
-  - rewrite lookup_ne.
-    apply Map.find_1.
-    apply MapFacts.add_neq_mapsto_iff; auto.
-    pose proof H x_ T_0 H1.
-    apply Map.find_2.
-    assumption.
-Qed.
-
-Lemma subG_add_2: forall G0 G1 y T_,
-  subG G0 G1 ->
-  Map.find y G0 = Some T_ ->
-  subG G0 (Map.add y T_ G1).
-Proof.
-  intros.
-  intros ?x_ ?T_ ?.
-
-  destruct (eq_x y x_); subst.
-  - rewrite H0 in H1.
-    inv H1.
-    apply Map.find_1.
-    now apply Map.add_1.
-  - apply Map.find_1.
-    apply MapFacts.add_neq_mapsto_iff; auto.
-    pose proof H x_ T_0 H1.
-    apply Map.find_2.
-    assumption.
+  - now rewrite H0, lookup_insert.
+  - now rewrite lookup_insert_ne.
 Qed.
 
 (* this is stricter than the ABS paper *)
 (* we require that any variables in the typing context also exist in the state *)
 Definition G_vdash_s (G5 : G) (s5 : s) :=
  forall (x5 : x) (T5 : T),
-  Map.find x5 G5 = Some (ctxv_T T5) ->
+  lookup x5 G5 = Some (ctxv_T T5) ->
   exists t5,
-  Map.find x5 s5 = Some t5 /\ typ_e G5 (e_t t5) T5.
+  lookup x5 s5 = Some t5 /\ typ_e G5 (e_t t5) T5.
 
 Notation "G1 G⊢ s1" := (G_vdash_s G1 s1) (at level 5).
 
 Lemma fresh_subG: forall G0 s0 (sub_list: list (T*x*t*x)),
   G_vdash_s G0 s0 ->
   fresh_vars_s (map (fun '(_,_,_,y)=>y) sub_list) s0 ->
-  NoDup (map (fun '(_,_,_,y)=>y) sub_list) ->
-  subG G0 (fold_right (fun '(T_,_,_,y_) G0 => Map.add y_ (ctxv_T T_) G0) G0 sub_list).
+  base.NoDup (map (fun '(_,_,_,y)=>y) sub_list) ->
+  subseteq G0 (fold_right (fun '(T_,_,_,y_) G0 => insert y_ (ctxv_T T_) G0) G0 sub_list).
 Proof.
   intros.
   induction sub_list.
@@ -94,15 +62,15 @@ Proof.
     pose proof IHsub_list H2 H5.
     cbn.
     apply subG_add; auto.
+    apply not_elem_of_dom_2 in H1.
+    apply not_elem_of_dom_1.
     intro.
-
-    apply MapFacts.in_find_iff in H3.
-    apply MapFacts.not_find_in_iff in H1.
-    pose proof map_neq_none_is_some _ _ H3 as (?T_, ?).
-    pose proof vars_well_typed _ _ _ H6 as (?T_, ->).
-    pose proof H _ _ H6 as (?t_, (?, _)).
-    rewrite H1 in H7.
-    discriminate.
+    apply elem_of_dom in H3.
+    inv H3.
+    destruct (vars_well_typed _ _ _ H6); subst.
+    apply H1.
+    pose proof H _ _ H6 as (t, (?, ?)).
+    apply elem_of_dom; auto.
 Qed.
 
 Lemma fresh_consistent: forall G0 s0 (sub_list: list (T*x*t*x)),
@@ -110,9 +78,9 @@ Lemma fresh_consistent: forall G0 s0 (sub_list: list (T*x*t*x)),
   (forall T_ t_, In (T_, t_) (map (fun '(T_, _, t_, _) => (T_, t_)) sub_list) ->
             typ_e G0 (e_t t_) T_) ->
   fresh_vars_s (map (fun '(_,_,_,y)=>y) sub_list) s0 ->
-  NoDup (map (fun '(_,_,_,y)=>y) sub_list) ->
-  G_vdash_s (fold_right (fun '(T_,_,_,y_) G0 => Map.add y_ (ctxv_T T_) G0) G0 sub_list)
-    (fold_right (fun '(_,_,t_,y_) s0 => Map.add y_ t_ s0) s0 sub_list).
+  base.NoDup (map (fun '(_,_,_,y)=>y) sub_list) ->
+  G_vdash_s (fold_right (fun '(T_,_,_,y_) G0 => insert y_ (ctxv_T T_) G0) G0 sub_list)
+    (fold_right (fun '(_,_,t_,y_) s0 => insert y_ t_ s0) s0 sub_list).
 Proof.
   intros.
   induction sub_list.
@@ -125,25 +93,18 @@ Proof.
     intros ?y ?T_ ?.
     destruct (eq_x y y0); subst.
   - exists t_.
-    split...
-    + apply Map.find_1.
-      now apply Map.add_1.
-    + assert (T_ = T_0).
-      {
-        apply Map.find_2 in H1.
-        apply MapFacts.add_mapsto_iff in H1.
-        destruct H1 as [(_, ?) | (?, ?)].
-        + now inv H1.
-        + exfalso.
-          now apply H1.
-      }
-      assert (In (T_0, t_) (map (fun '(T_, _, t_, _) => (T_, t_)) ((T_, x_, t_, y0) :: sub_list)))
-        by (left; now rewrite H2).
+    split; eauto with simpl_map.
+    assert (T_ = T_0).
+    {
+      simpl_map.
+      now inv H1.
+    }
+
+    assert (In (T_0, t_) (map (fun '(T_, _, t_, _) => (T_, t_)) ((T_, x_, t_, y0) :: sub_list)))
+      by (left; now rewrite H2).
       specialize (H0 _ _ H5).
       inv H0; constructor.
-  - apply Map.find_2 in H1.
-    apply Map.add_3 in H1; auto.
-    apply Map.find_1 in H1.
+  - simpl_map.
     assert (forall (T_ : T) (t_ : t),
              In (T_, t_) (map (fun '(T_0, _, t_0, _) => (T_0, t_0)) sub_list) ->
              typ_e G0 (e_t t_) T_).
@@ -155,20 +116,16 @@ Proof.
     }
     pose proof IHsub_list H2 H4 H7 _ _ H1 as (?t_, (?, ?)).
     exists t_0.
-    split...
-    + apply Map.find_1.
-      apply Map.add_2; auto.
-      apply Map.find_2; assumption.
-    + inv H8; constructor.
+    split; auto with simpl_map.
+    inv H8; constructor.
 Qed.
 
 Lemma subG_consistent: forall G1 G2 s0,
-  subG G1 G2 -> G_vdash_s G2 s0 -> G_vdash_s G1 s0.
+  subseteq G1 G2 -> G_vdash_s G2 s0 -> G_vdash_s G1 s0.
 Proof.
   intros.
-  intros x_ t_ ?.
-
-  pose proof H _ _ H1.
+  intros x_ T_ ?.
+  pose proof lookup_weaken _ _ _ _ H1 H.
   pose proof H0 _ _ H2 as (?t, (?, ?)).
   exists t.
   split; auto.
@@ -176,98 +133,26 @@ Proof.
 Qed.
 
 Lemma subG_type: forall G1 G2 e0 T0,
-  subG G1 G2 -> typ_e G1 e0 T0 -> typ_e G2 e0 T0.
+  subseteq G1 G2 -> typ_e G1 e0 T0 -> typ_e G2 e0 T0.
 Proof.
   intros.
   induction H0.
   - constructor.
   - constructor.
-  - apply H in H0.
-    constructor.
-    apply H0.
+  - constructor.
+    eapply lookup_weaken; eauto.
   - constructor.
     + intros.
       apply H1; auto.
-    + apply H in H2.
-      apply H2.
-Qed.
-
-(* this is 9.3.8 from Types and Programming Languages *)
-(* it has not yet proven useful *)
-Lemma subst_lemma_one_alt: forall (x0 x1:x) G0 e0 T0 T1,
-  typ_e (Map.add x0 (ctxv_T T1) G0) e0 T0 ->
-  typ_e G0 (e_var x1) T1 ->
-  typ_e G0 (e_var_subst_one e0 x0 x1) T0.
-Proof.
-  intros.
-  generalize dependent T0.
-  generalize dependent T1.
-  generalize dependent G0.
-  eapply e_ott_ind with
-      (n:=e0)
-      (P_list_e:= fun e_list => forall e0,
-                    In e0 e_list ->
-                    forall G0 T0 T1,
-                    typ_e (Map.add x0 (ctxv_T T1) G0) e0 T0 ->
-                    typ_e G0 (e_var x1) T1 ->
-                    typ_e G0 (e_var_subst e0 [(x0, x1)]) T0)
-  ;cbn; intros.
-  - inv H; simp e_var_subst_one; constructor.
-  - inv H.
-    simp e_var_subst_one.
-    destruct (eq_x x5 x0); subst.
-    + apply Map.find_2 in H3.
-      apply MapFacts.add_mapsto_iff in H3.
-      destruct H3 as [(?&?) | (?&?)]; subst.
-      * inv H1.
-        assumption.
-      * contradiction.
-    + constructor.
-      apply Map.find_1.
-      eapply Map.add_3.
-      * apply not_eq_sym.
-        apply n.
-      * apply Map.find_2 in H3.
-        apply H3.
-  - inv H1.
-    simp e_var_subst_one.
-    rewrite <- subst_fst_commute.
-    replace (map (fun x : e * T => let (e_, _) := let '(e_, T_) := x in (e_var_subst_one e_ x0 x1, T_) in e_) e_T_list)
-      with
-        (map (fun pat_ : e * T => let (e_, _) := pat_ in e_)
-           (map (fun '(e_, T_) => (e_var_subst_one e_ x0 x1, T_)) e_T_list))
-    by apply map_map.
-    constructor.
-    + rewrite map_map.
-      intros.
-      apply in_map_iff in H1.
-      destruct H1 as ((?e_&?T_) & ? & ?).
-      inv H1.
-      eapply H.
-      * apply in_map_iff.
-        exists (e_0, T_).
-        split; eauto.
-      * apply H5.
-        apply in_map_iff.
-        exists (e_0, T_).
-        split; auto.
-      * apply H0.
-    + apply Map.find_1.
-      apply Map.find_2 in H7.
-      rewrite subst_snd_commutes.
-      eapply Map.add_3; eauto.
-  - inv H.
-  - inv H1.
-    + eapply H; eauto.
-    + eapply H0; eauto.
+    + eapply lookup_weaken; eauto.
 Qed.
 
 Lemma same_type_sub: forall (sub_list: list (x*x)) G0 e0 T0,
     typ_e G0 e0 T0 ->
     (forall x0 y0 T0,
       In (x0, y0) sub_list ->
-      Map.find x0 G0 = Some T0 ->
-      Map.find y0 G0 = Some T0) ->
+      lookup x0 G0 = Some T0 ->
+      lookup y0 G0 = Some T0) ->
     typ_e G0 (e_var_subst e0 sub_list) T0.
 Proof.
   {
@@ -334,9 +219,9 @@ Proof.
 Qed.
 
 Lemma subst_lemma_one: forall G0 x0 y0 e0 Ai A,
-  typ_e (Map.add x0 Ai G0) e0 A ->
+  typ_e (insert x0 Ai G0) e0 A ->
   fresh_vars_e [y0] e0 ->
-  typ_e (Map.add y0 Ai G0) (e_var_subst_one e0 x0 y0) A.
+  typ_e (insert y0 Ai G0) (e_var_subst_one e0 x0 y0) A.
 Proof.
   {
     intros.
@@ -348,20 +233,18 @@ Proof.
                       forall e0 A,
                       In e0 e_list ->
                       fresh_vars_e [y0] e0 ->
-                      typ_e (Map.add x0 Ai G0) e0 A ->
-                      typ_e (Map.add y0 Ai G0) (e_var_subst_one e0 x0 y0) A);
+                      typ_e (insert x0 Ai G0) e0 A ->
+                      typ_e (insert y0 Ai G0) (e_var_subst_one e0 x0 y0) A);
       intros.
     - simp e_var_subst_one.
       inv H; constructor.
     - simp e_var_subst_one.
       inv H.
-      apply Map.find_2 in H3.
-      apply MapFacts.add_mapsto_iff in H3.
+      apply lookup_insert_Some in H3.
       destruct H3 as [(?,?)|(?,?)]; subst.
       + destruct (eq_x x5 x5); subst.
         * constructor.
-          apply Map.find_1.
-          now apply Map.add_1.
+          now simpl_map.
         * contradiction.
 
       + destruct (eq_x x5 x0); subst.
@@ -372,8 +255,7 @@ Proof.
              apply H0.
              now left.
           -- constructor.
-             apply Map.find_1.
-             apply Map.add_2; eauto.
+             now simpl_map.
     - simp e_var_subst_one.
       inv H1.
       replace (e_list_subst_one (map (fun pat_ : e * T => let (e_, _) := pat_ in e_) e_T_list) x0 y0)
@@ -407,14 +289,7 @@ Proof.
       + replace (map (fun pat_ : e * T => let (_, T_) := pat_ in T_) (map (fun '(e, T) => (e_var_subst_one e x0 y0, T)) e_T_list))
           with(map (fun pat_ : e * T => let (_, T_) := pat_ in T_) e_T_list)
           by (rewrite map_map; apply map_ext; now intros (?, ?)).
-
-        apply Map.find_2 in H7.
-        apply MapFacts.add_mapsto_iff in H7.
-        destruct H7 as [(?,?)|(?,?)].
-        * exfalso.
-          apply (vars_fs_distinct _ _ H1).
-        * apply Map.find_1.
-          apply Map.add_2; eauto.
+        now simpl_map.
     - inv H.
     - destruct H1; subst.
       + apply H; eauto.
@@ -422,31 +297,18 @@ Proof.
   }
 Qed.
 
-Lemma typ_e_G_Equal_equiv_imp : 
- forall G1 G2 e T, Map.Equal G1 G2 -> typ_e G1 e T -> typ_e G2 e T.
+Lemma typ_e_G_Equal_equiv_imp :
+ forall G1 G2 e T, G1 = G2 -> typ_e G1 e T -> typ_e G2 e T.
 Proof.
 intros G1 G2 e0 T0 Heq.
 intros Ht.
-induction Ht.
-- apply typ_bool.
-- apply typ_int.
-- apply typ_var.
-  symmetry in Heq.
-  rewrite <- H.
-  apply Heq.
-- apply typ_func_expr.
-  * intros.
-    apply H0; auto.
-  * rewrite <- H1.
-    symmetry in Heq.
-    apply Heq.
+now rewrite <- Heq.
 Qed.
 
-Lemma typ_e_G_Equal_equiv : 
- forall G1 G2 e T, Map.Equal G1 G2 -> (typ_e G1 e T <-> typ_e G2 e T).
+Lemma typ_e_G_Equal_equiv :
+ forall G1 G2 e T, G1 = G2 -> (typ_e G1 e T <-> typ_e G2 e T).
 Proof.
 intros G1 G2 e0 T0 Heq; split; apply typ_e_G_Equal_equiv_imp; auto.
-symmetry; assumption.
 Qed.
 
 Lemma fold_map4 {A X Y Z W: Type}: forall (f : _ -> _ -> A -> A) (l: list (X*Y*Z*W)) a0,
@@ -472,12 +334,12 @@ Proof.
 Qed.
 
 Lemma subst_lemma: forall (T_x_t_y_list:list (T*x*t*x)) G0 e0 A,
-  typ_e (fold_right (fun '(Ai, x_, _, _) (G0 : G) => Map.add x_ (ctxv_T Ai) G0) G0 T_x_t_y_list) e0 A ->
-  NoDup (map (fun '(_, _, _, y) => y) T_x_t_y_list) ->
-  NoDup (map (fun '(_, x, _, _) => x) T_x_t_y_list) ->
+  typ_e (fold_right (fun '(Ai, x_, _, _) (G0 : G) => insert x_ (ctxv_T Ai) G0) G0 T_x_t_y_list) e0 A ->
+  base.NoDup (map (fun '(_, _, _, y) => y) T_x_t_y_list) ->
+  base.NoDup (map (fun '(_, x, _, _) => x) T_x_t_y_list) ->
   fresh_vars_e (map (fun '(_, _, _, y) => y) T_x_t_y_list) e0 ->
   disjoint (map (fun '(_, _, _, y) => y) T_x_t_y_list) (map (fun '(_, x, _, _) => x) T_x_t_y_list) ->
-  typ_e (fold_right (fun '(Ai, _, _, y) (G0 : G) => Map.add y (ctxv_T Ai) G0) G0 T_x_t_y_list)
+  typ_e (fold_right (fun '(Ai, _, _, y) (G0 : G) => insert y (ctxv_T Ai) G0) G0 T_x_t_y_list)
     (e_var_subst e0 (map (fun '(_, x_, _, y_) => (x_, y_)) T_x_t_y_list)) A.
 Proof.
   intros.
@@ -513,7 +375,7 @@ Proof.
       rewrite map_map in H10.
       revert H10.
       clear.
-      induction T_x_t_y_list; auto.
+      induction T_x_t_y_list; try easy.
       simpl.
       intros Hx.
       destruct Hx.
@@ -524,18 +386,18 @@ Proof.
         apply IHT_x_t_y_list.
         assumption.
     }
-    assert (Map.Equal
-     (Map.add x_ (ctxv_T T_) (fold_right (fun '(Ai, x_0, _, _) (G0 : G) => Map.add x_0 (ctxv_T Ai) G0) G0 T_x_t_y_list))
-     (fold_right (fun '(Ai, x_, _, _) (G0 : G) => Map.add x_ (ctxv_T Ai) G0) (Map.add x_ (ctxv_T T_) G0) T_x_t_y_list))
+    assert ((insert x_ (ctxv_T T_) (fold_right (fun '(Ai, x_0, _, _) (G0 : G) => insert x_0 (ctxv_T Ai) G0) G0 T_x_t_y_list))
+              =
+     (fold_right (fun '(Ai, x_, _, _) (G0 : G) => insert x_ (ctxv_T Ai) G0) (insert x_ (ctxv_T T_) G0) T_x_t_y_list))
       as HMEqualx.
     {
+      simplify_map_eq.
       epose proof fold_add_comm G0 x_ T_ (map (fun '(Ai, x1, _, _) => (Ai, x1)) T_x_t_y_list) Hinx.
       rewrite 2 fold_map4.
       assumption.
     }
-    assert (Map.Equal
-     (fold_right (fun '(Ai, _, _, y) (G0 : G) => Map.add y (ctxv_T Ai) G0) (Map.add x_ (ctxv_T T_) G0) T_x_t_y_list)
-     (Map.add x_ (ctxv_T T_) (fold_right (fun '(Ai, _, _, y) (G0 : G) => Map.add y (ctxv_T Ai) G0) G0 T_x_t_y_list)))
+    assert ((fold_right (fun '(Ai, _, _, y) (G0 : G) => insert y (ctxv_T Ai) G0) (insert x_ (ctxv_T T_) G0) T_x_t_y_list) =
+     (insert x_ (ctxv_T T_) (fold_right (fun '(Ai, _, _, y) (G0 : G) => insert y (ctxv_T Ai) G0) G0 T_x_t_y_list)))
       as HMEqualy.
     {
       epose proof fold_add_comm G0 x_ T_ (map (fun '(Ai, _, _, y1) => (Ai, y1)) T_x_t_y_list) H9.
@@ -547,7 +409,7 @@ Proof.
       assumption.
     }
     apply (typ_e_G_Equal_equiv _ _ _ _ HMEqualx) in H.
-    pose proof IHT_x_t_y_list H7 H8 H4 _ H1 _ H as IH.
+    epose proof IHT_x_t_y_list H7 H8 H4 _ H1 _ H as IH.
     apply (typ_e_G_Equal_equiv _ _ _ _ HMEqualy) in IH.
     assert (fresh_vars_e [y] (e_var_subst e0 (map (fun '(_, x_, _, y_) => (x_, y_)) T_x_t_y_list))).
     {
@@ -558,6 +420,9 @@ Proof.
         now intros (((?, ?), ?), ?).
       }
       apply fresh_var_subst; try rewrite H10; auto.
+      intro.
+      apply H6.
+      apply elem_of_list_In; auto.
     }
     now apply (subst_lemma_one _ _ _ _ _ _ IH H10).
 Qed.
@@ -568,7 +433,7 @@ Lemma type_preservation : forall (Flist : list F) (G5 : G) (s5 : s),
   forall (e5 : e) (T5 : T) (s' : s) (e' : e),
     typ_e G5 e5 T5 ->
     red_e Flist s5 e5 s' e' ->
-    exists G', subG G5 G' /\ G_vdash_s G' s' /\ typ_e G' e' T5.
+    exists G', subseteq G5 G' /\ G_vdash_s G' s' /\ typ_e G' e' T5.
 Proof.
   intros Fs G5 s0 s_well_typed F_well_typed.
   intros e0 T0 s' e' e0_type reduction.
@@ -663,8 +528,7 @@ Proof.
            simpl.
            lia.
       * rewrite combine_snd.
-        ++ apply G'extends.
-           apply H4.
+        ++ eapply lookup_weaken; eauto.
         ++ rewrite map_length.
            rewrite H3.
            rewrite 2 combine_app; auto.
@@ -713,22 +577,25 @@ Proof.
         intros.
         now destruct a as (((?, ?), ?), ?).
     }
-    exists (fold_right (fun '(T_, _, _, y) G0 => Map.add y (ctxv_T T_) G0) G5 T_x_t_y_list).
+    exists (fold_right (fun '(T_, _, _, y) G0 => insert y (ctxv_T T_) G0) G5 T_x_t_y_list).
     splits.
     + eapply fresh_subG; eauto.
-    + rewrite <- fold_map.
-      apply fresh_consistent; eauto.
-      intros.
-      apply in_map_iff in H12.
-      destruct H12 as (Txty, (?, ?)).
-      apply H6.
-      inv H12.
-      rewrite map_map.
-      apply in_map_iff.
-      exists Txty.
-      split; auto.
-      destruct Txty as (((?, ?), ?), ?).
-      now inv H15.
+    +
+      (* now what??*)
+      Fail rewrite <- fold_map.
+      admit.
+      (* apply fresh_consistent; eauto. *)
+      (* intros. *)
+      (* apply in_map_iff in H12. *)
+      (* destruct H12 as (Txty, (?, ?)). *)
+      (* apply H6. *)
+      (* inv H12. *)
+      (* rewrite map_map. *)
+      (* apply in_map_iff. *)
+      (* exists Txty. *)
+      (* split; auto. *)
+      (* destruct Txty as (((?, ?), ?), ?). *)
+      (* now inv H15. *)
 
     + rewrite H7 in H11.
       inv H11.
@@ -736,5 +603,5 @@ Proof.
       * rewrite <- fold_map_reshuffle; eauto.
       * rewrite map_xs in H10.
         apply H10.
-Qed.
+Admitted.
 End FunctionalMetatheory.
